unambiguous decomposition of CDDL array groups

src/cbor/CDDL.Spec.fsti
@@ -287,10 +287,163 @@ let array_group3_concat_equiv
   (ensures ((a1 `array_group3_concat` a2) `array_group3_equiv` (a1' `array_group3_concat` a2')))
 = ()
 
+let array_group3_concat_unique
+  #b (a1 a3: array_group3 b)
+: Tot prop
+= forall (l1 l2: (l: list Cbor.raw_data_item { opt_precedes_list l b })) .
+    Some? (a3 l2) ==> (a1 l1 == Some (l1, []) <==> a1 (l1 `List.Tot.append` l2) == Some (l1, l2))
+
+let array_group3_concat_unique_prop_intro
+  #b (a1 a3: array_group3 b)
+  (l1 l2: (l: list Cbor.raw_data_item { opt_precedes_list l b }))
+  (l3 rem: list Cbor.raw_data_item)
+: Lemma
+  (requires (
+    array_group3_concat_unique a1 a3 /\
+    (a1 l1 == Some (l1, []) /\ a3 l2 == Some (l3, rem))
+  ))
+  (ensures (
+      array_group3_concat a1 a3 (l1 `List.Tot.append` l2) == Some (l1 `List.Tot.append` l3, rem)
+  ))
+= ()
+
+let array_group3_concat_unique_prop_elim_gen
+  #b (a1 a3: array_group3 b)
+  (l: list Cbor.raw_data_item { opt_precedes_list l b })
+  (l' rem: list Cbor.raw_data_item)
+: Lemma
+  (requires (
+    array_group3_concat_unique a1 a3 /\
+    array_group3_concat a1 a3 l == Some (l', rem)
+  ))
+  (ensures (
+      (exists (l1 l2 l3: list Cbor.raw_data_item) .
+        a1 l == Some (l1, l2) /\
+        a1 l1 == Some (l1, []) /\
+        a3 l2 == Some (l3, rem) /\
+        l' == l1 `List.Tot.append` l3
+  )))
+= ()
+
+let array_group3_concat_unique_prop_elim
+  #b (a1 a3: array_group3 b)
+  (l: list Cbor.raw_data_item { opt_precedes_list l b })
+: Lemma
+  (requires (
+    array_group3_concat_unique a1 a3 /\
+    array_group3_concat a1 a3 l == Some (l, [])
+  ))
+  (ensures (
+      (exists (l1 l2: list Cbor.raw_data_item) .
+        a1 l == Some (l1, l2) /\
+        a1 l1 == Some (l1, []) /\
+        a3 l2 == Some (l2, []))
+  ))
+= array_group3_concat_unique_prop_elim_gen a1 a3 l l [];
+  let Some (l1, l2) = a1 l in
+  let Some (l3, _) = a3 l2 in
+  List.Tot.append_l_nil l3
+
+let array_group3_strong_prefix
+  #b (a1: array_group3 b)
+: Tot prop
+= forall (l1 l2: (l: list Cbor.raw_data_item { opt_precedes_list l b })) .
+    (a1 l1 == Some (l1, []) <==> a1 (l1 `List.Tot.append` l2) == Some (l1, l2))
+
+let array_group3_strong_prefix_empty
+  (b: option Cbor.raw_data_item)
+: Lemma
+  (array_group3_strong_prefix #b array_group3_empty)
+= ()
+
+let array_group3_strong_prefix_implies_concat_unique
+  #b (a1 a3: array_group3 b)
+: Lemma
+  (array_group3_strong_prefix a1 ==> array_group3_concat_unique a1 a3)
+= ()
+
+let array_group3_concat_unique_strong_prefix
+  #b (a1 a2: array_group3 b)
+: Lemma
+  (requires (
+    array_group3_concat_unique a1 a2 /\
+    array_group3_strong_prefix a2
+  ))
+  (ensures (
+    array_group3_strong_prefix (array_group3_concat a1 a2)
+  ))
+= let a = array_group3_concat a1 a2 in
+  let prf
+    (l1 l2: (l: list Cbor.raw_data_item { opt_precedes_list l b }))
+  : Lemma
+    (a l1 == Some (l1, []) ==> a (l1 `List.Tot.append` l2) == Some (l1, l2))
+  = if FStar.StrongExcludedMiddle.strong_excluded_middle (a l1 == Some (l1, []))
+    then begin
+      let Some (l11, l12) = a1 l1 in
+      List.Tot.append_assoc l11 l12 l2
+    end
+    else ()
+  in
+  Classical.forall_intro_2 prf
+
+let array_group3_concat_unique_concat
+  #b (a1 a2 a3: array_group3 b)
+: Lemma
+  (requires (
+    array_group3_concat_unique a1 a2
+  ))
+  (ensures (
+    array_group3_concat_unique a1 (array_group3_concat a2 a3)
+  ))
+= ()
+
 let array_group3_choice #b (a1 a3: array_group3 b) : array_group3 b =
   fun l -> match a1 l with
     | None -> a3 l
     | Some l3 -> Some l3
+
+let array_group3_concat_unique_choice_right #b (a1 a2 a3: array_group3 b) : Lemma
+  (requires (
+    array_group3_concat_unique a1 a2 /\
+    array_group3_concat_unique a1 a3
+  ))
+  (ensures (
+    array_group3_concat_unique a1 (array_group3_choice a2 a3)
+  ))
+= ()
+
+let array_group3_disjoint #b (a1 a2: array_group3 b) : Tot prop
+= (forall (l: list Cbor.raw_data_item { opt_precedes_list l b }) . ~ (Some? (a1 l) /\ Some? (a2 l)))
+
+let array_group3_concat_unique_choice_left #b (a1 a2 a3: array_group3 b) : Lemma
+  (requires (
+    array_group3_concat_unique a1 a3 /\
+    array_group3_concat_unique a2 a3 /\
+    array_group3_disjoint a1 a2
+  ))
+  (ensures (
+    array_group3_concat_unique (array_group3_choice a1 a2) a3
+  ))
+= ()
+
+let array_group3_disjoint_sym #b (a1 a2: array_group3 b) : Lemma
+  (array_group3_disjoint a1 a2 <==> array_group3_disjoint a2 a1)
+= ()
+
+let array_group3_disjoint_choice #b (a1 a2 a3: array_group3 b) : Lemma
+  (requires (
+    array_group3_disjoint a1 a2 /\
+    array_group3_disjoint a1 a3
+  ))
+  (ensures (
+    array_group3_disjoint a1 (array_group3_choice a2 a3)
+  ))
+= ()
+
+let array_group3_disjoint_concat #b (a1 a2 a3: array_group3 b) : Lemma
+  (requires (array_group3_disjoint a1 a2))
+  (ensures (array_group3_disjoint a1 (array_group3_concat a2 a3)))
+= ()
 
 let rec array_group3_zero_or_more' #b (a: array_group3 b) (l: list Cbor.raw_data_item { opt_precedes_list l b }) : Ghost (option (list Cbor.raw_data_item & list Cbor.raw_data_item))
   (requires True)
@@ -310,6 +463,99 @@ let rec array_group3_zero_or_more' #b (a: array_group3 b) (l: list Cbor.raw_data
       end
 
 let array_group3_zero_or_more #b : array_group3 b -> array_group3 b = array_group3_zero_or_more'
+
+let rec array_group3_zero_or_more_some
+  #b
+  (a: array_group3 b)
+  (l: list Cbor.raw_data_item { opt_precedes_list l b })
+: Lemma
+  (ensures (Some? (array_group3_zero_or_more a l)))
+  (decreases List.Tot.length l)
+  [SMTPat (array_group3_zero_or_more a l)]
+= match a l with
+  | None -> ()
+  | Some (l1, l2) ->
+    List.Tot.append_length l1 l2;
+    if Nil? l1
+    then ()
+    else array_group3_zero_or_more_some a l2
+
+let array_group3_concat_unique_concat_zero_or_more_right
+  #b (a1 a2 a3: array_group3 b)
+: Lemma
+  (requires (
+    array_group3_concat_unique a1 a2 /\
+    array_group3_concat_unique a1 a3
+  ))
+  (ensures (
+    array_group3_concat_unique a1 (array_group3_concat (array_group3_zero_or_more a2) a3)
+  ))
+= ()
+
+let array_group3_concat_unique_zero_or_more_right
+  #b (a1 a2: array_group3 b)
+: Lemma
+  (ensures (
+    array_group3_concat_unique a1 (array_group3_zero_or_more a2) <==> array_group3_strong_prefix a1
+  ))
+= ()
+
+let array_group3_concat_unique_zero_or_more_left
+  #b (a1 a2: array_group3 b)
+: Lemma
+  (requires (
+    array_group3_disjoint a1 a2 /\
+    array_group3_concat_unique a1 a1 /\
+    array_group3_concat_unique a1 a2
+  ))
+  (ensures (
+    array_group3_concat_unique (array_group3_zero_or_more a1) a2
+  ))
+= let _ : squash (array_group3_disjoint a1 a2) = () in
+  let rec prf
+    (l1 l2: (l: list Cbor.raw_data_item { opt_precedes_list l b }))
+  : Lemma
+    (ensures (
+      Some? (a2 l2) ==> (array_group3_zero_or_more a1 l1 == Some (l1, []) <==> array_group3_zero_or_more a1 (l1 `List.Tot.append` l2) == Some (l1, l2))
+    ))
+    (decreases (List.Tot.length l1))
+  = if Some? (a2 l2)
+    then begin
+      if FStar.StrongExcludedMiddle.strong_excluded_middle (array_group3_zero_or_more a1 l1 == Some (l1, []))
+      then
+        match a1 l1 with
+        | None -> ()
+        | Some (l1l, l1r) ->
+          if Nil? l1l
+          then ()
+          else begin
+            List.Tot.append_length l1l l1r;
+            List.Tot.append_assoc l1l l1r l2;
+            let Some (l1rl, l1rr) = array_group3_zero_or_more a1 l1r in
+            assert (Nil? l1rr);
+            List.Tot.append_l_nil l1rl;
+            prf l1r l2
+          end
+      else if FStar.StrongExcludedMiddle.strong_excluded_middle (array_group3_zero_or_more a1 (l1 `List.Tot.append` l2) == Some (l1, l2))
+      then begin
+        match a1 (l1 `List.Tot.append` l2) with
+        | None -> ()
+        | Some (l12l, l12r) ->
+          let Some (l12rl, l12rr) = array_group3_zero_or_more a1 l12r in
+          assert (l12rr == l2);
+          List.Tot.append_assoc l12l l12rl l2;
+          List.Tot.append_length l12rl l12rr;
+          List.Tot.append_length l12l l12r;
+          List.Tot.append_length l1 l2;
+          if Nil? l12l
+          then ()
+          else begin
+            prf l12rl l2
+          end
+      end
+    end
+  in
+  Classical.forall_intro_2 prf
 
 let array_group3_one_or_more #b (a: array_group3 b) : array_group3 b =
   a `array_group3_concat` array_group3_zero_or_more a
